added Hoskinson

src/Hoskinson.lean
@@ -1,31 +1,35 @@
-namespace Typesig
+import Lean
+namespace Hoskinson
 
 #eval Lean.versionString
 
 set_option pp.notation true
+set_option pp.rawOnError true
 set_option hygiene false
 set_option maxRecDepth 1000000
 set_option maxHeartbeats 1000000
 
 inductive Tp : Type where
-| natural : Tp
-| function : Tp → Tp → Tp
+  | natural : Tp
+  | function : Tp → Tp → Tp
+  deriving Repr, Inhabited, DecidableEq
 
 notation:max "ℕ" => Tp.natural
-infixr:70 "⇒" => Tp.function
+infixr:70 " ⇒ " => Tp.function
 
 example : Tp := ℕ ⇒ ℕ
 
 inductive TpEnv : Type where
-| empty : TpEnv
-| extend : TpEnv → Tp → TpEnv
+  | empty : TpEnv
+  | extend : TpEnv → Tp → TpEnv
+  deriving Repr, Inhabited, DecidableEq
 
 notation:max "∅" => TpEnv.empty
-infixl:50 "▷" => TpEnv.extend
+infixl:50 " ▷ " => TpEnv.extend
 
 example : TpEnv := ∅ ▷ ℕ ⇒ ℕ ▷ ℕ
 
-infix:40  "∋" => lookup
+infix:40  " ∋ " => lookup
 
 inductive lookup : TpEnv → Tp → Type where
   | stop :
@@ -35,12 +39,12 @@ inductive lookup : TpEnv → Tp → Type where
        Γ ∋ B
        ----------------
      → Γ ▷ A ∋ B
-  deriving Repr
+  deriving Repr, DecidableEq
 
 prefix:90 "S" => lookup.pop
 notation:max "Z" => lookup.stop
 
-infix:40  "⊢" => term
+infix:40  " ⊢ " => term
 
 inductive term : TpEnv → Tp → Type where
   | var :
@@ -75,65 +79,59 @@ inductive term : TpEnv → Tp → Type where
       → Γ ⊢ A
   deriving Repr
 
-prefix:90 "#" => term.var
-prefix:50 "ƛ" => term.lambda
-infixl:70 "⬝" => term.application
+prefix:90 "# " => term.var
+prefix:50 "ƛ " => term.lambda
+infixl:70 " ⬝ " => term.application
 notation:max "o" => term.zero
-postfix:80 "+1" => term.succ
-notation:max "switch" => term.case
-prefix:50 "μ" => term.mu
+postfix:80 " +1" => term.succ
+notation:max "casesOn" => term.case
+prefix:50 "μ " => term.mu
 
 instance : OfNat (Γ ⊢ ℕ) Nat.zero where
-  ofNat := term.zero
+  ofNat := o
 
 instance [OfNat (Γ ⊢ ℕ) n] : OfNat (Γ ⊢ ℕ) (Nat.succ n) where
-  ofNat := term.succ (OfNat.ofNat n)
+  ofNat := (OfNat.ofNat n) +1
 
-example : 2 = @term.zero ∅ +1 +1 := rfl
+example : 2 = (o +1 +1 : ∅ ⊢ ℕ) := rfl
 
 instance : OfNat (Γ ▷ A ∋ A) Nat.zero where
-  ofNat := lookup.stop
+  ofNat := Z
 
 instance [OfNat (Γ ∋ B) n] : OfNat (Γ ▷ A ∋ B) (Nat.succ n) where
-  ofNat := lookup.pop (OfNat.ofNat n)
+  ofNat := S (OfNat.ofNat n)
 
 example : 2 = (S S Z : ∅ ▷ ℕ ⇒ ℕ ▷ ℕ ▷ ℕ ∋ ℕ ⇒ ℕ) := rfl
 
 def plus : Γ ⊢ ℕ ⇒ ℕ ⇒ ℕ :=
-  μ ƛ ƛ (switch (# Z) (# S Z) ((# S S S Z ⬝ # S S Z ⬝ # Z) +1))
+  -- μ ƛ ƛ (casesOn (# Z) (# S Z) ((# S S S Z ⬝ # S S Z ⬝ # Z) +1))
+  μ ƛ ƛ (casesOn (# 0) (# 1) ((# 3 ⬝ # S S Z ⬝ # Z) +1))
 def two_plus_two : ∅ ⊢ ℕ :=
   plus ⬝ 2 ⬝ 2
 
-def one_c : ∅ ⊢ (A ⇒ A) ⇒ A ⇒ A := ƛ ƛ # S Z ⬝ # Z
-def one_c' : ∅ ⊢ (A ⇒ A) ⇒ A ⇒ A := ƛ ƛ # 1 ⬝ (# 0 : _ ⊢ A)
-
--- suc = ƛ "m" ⇒ succ (# "m")
+def Ch (A : Tp) : Tp := (A ⇒ A) ⇒ A ⇒ A
 def suc_c : Γ ⊢ ℕ ⇒ ℕ :=
   ƛ (# Z +1)
-def Ch (A : Tp) : Tp := (A ⇒ A) ⇒ A ⇒ A
+-- twoᶜ =  ƛ "s" ⇒ ƛ "z" ⇒ # "s" · (# "s" · # "z")
 def two_c : Γ ⊢ Ch A :=
   ƛ ƛ (# S Z ⬝ (# S Z ⬝ # Z))
--- twoᶜ =  ƛ "s" ⇒ ƛ "z" ⇒ # "s" · (# "s" · # "z")
+-- plusᶜ =  ƛ "m" ⇒ ƛ "n" ⇒ ƛ "s" ⇒ ƛ "z" ⇒ # "m" · # "s" · (# "n" · # "s" · # "z")
 def plus_c : Γ ⊢ Ch A ⇒ Ch A ⇒ Ch A :=
   ƛ ƛ ƛ ƛ (# S S S Z ⬝ # S Z ⬝ (# S S Z ⬝ # S Z ⬝ # Z))
 def plus_c' : Γ ⊢ Ch A ⇒ Ch A ⇒ Ch A :=
   ƛ ƛ ƛ ƛ ((# 3 : _ ⊢ Ch A) ⬝ # 1 ⬝ ((# 2 : _ ⊢ Ch A) ⬝ # 1 ⬝ # 0))
--- plusᶜ =  ƛ "m" ⇒ ƛ "n" ⇒ ƛ "s" ⇒ ƛ "z" ⇒ # "m" · # "s" · (# "n" · # "s" · # "z")
 def two : ∅ ⊢ ℕ := two_c ⬝ suc_c ⬝ 0
-
 
 def rmap (Γ Δ : TpEnv) : Type :=
   ∀ {A : Tp}, (Γ ∋ A) → (Δ ∋ A)
-
 def smap (Γ Δ : TpEnv) : Type :=
   ∀ {A : Tp}, (Γ ∋ A) → (Δ ⊢ A)
-
 def tmap (Γ Δ : TpEnv) : Type :=
   ∀ {A : Tp}, (Γ ⊢ A) → (Δ ⊢ A)
 
-infix:30 "→ʳ" => rmap
-infix:30 "→ˢ" => smap
-infix:30 "→ᵗ" => tmap
+infix:30 " →ʳ " => rmap
+infix:30 " →ˢ " => smap
+infix:30 " →ᵗ " => tmap
 
 def ren_ext {Γ Δ : TpEnv} {A :Tp} (ρ : Γ →ʳ Δ) : (Γ ▷ A →ʳ Δ ▷ A)
   | _ , Z  =>  Z
@@ -145,8 +143,7 @@ def ren {Γ Δ : TpEnv} (ρ : Γ →ʳ Δ) : Γ →ᵗ Δ
   | _ , (L ⬝ M) => ren ρ L ⬝ ren ρ M
   | _ , o => o
   | _ , M +1 => ren ρ M +1
-  | _ , switch L M N =>
-        switch (ren ρ L) (ren ρ M) (ren (ren_ext ρ) N)
+  | _ , casesOn L M N => casesOn (ren ρ L) (ren ρ M) (ren (ren_ext ρ) N)
   | _ , μ N => μ (ren (ren_ext ρ) N)
 
 def lift {Γ : TpEnv} {A : Tp} : Γ →ᵗ Γ ▷ A := ren (fun x => S x)
@@ -161,8 +158,7 @@ def sub {Γ Δ : TpEnv} (σ : Γ →ˢ Δ) : Γ →ᵗ Δ
   | _ , (L ⬝ M) => sub σ L ⬝ sub σ M
   | _ , o => o
   | _ , M +1 => sub σ M +1
-  | _ , switch L M N =>
-        switch (sub σ L) (sub σ M) (sub (sub_ext σ) N)
+  | _ , casesOn L M N => casesOn (sub σ L) (sub σ M) (sub (sub_ext σ) N)
   | _ , μ N => μ (sub (sub_ext σ) N)
 
 def sigma_0 (M : Γ ⊢ A) : Γ ▷ A →ˢ Γ
@@ -183,9 +179,13 @@ inductive Value : Γ ⊢ A → Type where
       Value V → Value (V +1)
   deriving Repr
 
+open Value
+
+infix:30 "~>" => reduce
+
 inductive reduce : Γ ⊢ A → Γ ⊢ A → Type where
   | xi_app_1 :
-      reduce L L' → reduce (L ⬝ M) (L' ⬝ M)
+      L ~> L' → L ⬝ M ~> L' ⬝ M
   | xi_app_2 :
       Value V → reduce M M' → reduce (V ⬝ M) (V ⬝ M')
   | beta :
@@ -193,18 +193,17 @@ inductive reduce : Γ ⊢ A → Γ ⊢ A → Type where
   | xi_succ :
       reduce M M' → reduce (M +1) (M' +1)
   | xi_case :
-      reduce L L' → reduce (switch L M N) (switch L' M N)
+      reduce L L' → reduce (casesOn L M N) (casesOn L' M N)
   | beta_zero :
-      reduce (switch o M N) M
+      reduce (casesOn o M N) M
   | beta_succ :
-      Value V → reduce (switch (V +1) M N) (subst N V)
+      Value V → reduce (casesOn (V +1) M N) (subst N V)
   | beta_mu :
       reduce (μ N) (subst N (μ N))
   deriving Repr
 
 open reduce
 
-infix:20 "~>" => reduce
 
 -- inductive star : (Γ ⊢ A) → (Γ ⊢ A) → Type where
 --   | none :
@@ -224,16 +223,19 @@ infix:20 "~>" => reduce
 --                  (star : (Γ ⊢ A) → (Γ ⊢ A) → Type) where
 --   trans := star.two
 
+infix:30 "~>>"  => reduce_many
+
 inductive reduce_many : Γ ⊢ A → Γ ⊢ A → Type where
   | nil :
-      reduce_many M M
+      M ~>> M
   | cons :
-      ∀ L, reduce L M → reduce_many M N → reduce_many L N
+      ∀ L, L ~> M
+         → M ~>> N
+           -------
+         → L ~>> N
   deriving Repr
 
 open reduce_many
-
-infix:20 "~>>"  => reduce_many
 
 def one_one : (L ~> M) → (M ~> N) → (L ~>> N)
   | L_to_M, M_to_N => cons _ L_to_M (cons _ M_to_N nil)
@@ -270,28 +272,30 @@ instance : Trans (.~>>. : Γ ⊢ A → Γ ⊢ A → Type)
   trans := many_many
 
 example : two ~> (ƛ (suc_c ⬝ (suc_c ⬝ # Z))) ⬝ 0
-    := xi_app_1 (beta Value.lambda)
+    := xi_app_1 (beta lambda)
 
-example : ((ƛ (suc_c ⬝ (suc_c ⬝ # Z))) ⬝ 0 : ∅ ⊢ ℕ) ~> suc_c ⬝ (suc_c ⬝ 0)
-    := beta Value.zero
+example : (ƛ (suc_c ⬝ (suc_c ⬝ # Z))) ⬝ (0 : ∅ ⊢ ℕ) ~> suc_c ⬝ (suc_c ⬝ 0)
+    := beta zero
 
 example : (suc_c ⬝ (suc_c ⬝ 0) : ∅ ⊢ ℕ) ~> suc_c ⬝ 1
-    := xi_app_2 Value.lambda (beta Value.zero)
+    := xi_app_2 lambda (beta zero)
 
 example : (suc_c ⬝ 1 : ∅ ⊢ ℕ) ~> 2
-    := beta (Value.succ Value.zero)
+    := beta (succ zero)
 
-example : two ~>> 2 :=
+def two_to_2 :=
   calc
     (two_c ⬝ suc_c ⬝ 0 : ∅ ⊢ ℕ)
-      ~> (ƛ (suc_c ⬝ (suc_c ⬝ # Z))) ⬝ 0  := xi_app_1 (beta Value.lambda)
-    _ ~> (suc_c ⬝ (suc_c ⬝ 0))            := beta Value.zero
-    _ ~> suc_c ⬝ 1                        := xi_app_2 Value.lambda (beta Value.zero)
-    _ ~> 2                                := beta (Value.succ Value.zero)
+      ~> (ƛ (suc_c ⬝ (suc_c ⬝ # Z))) ⬝ 0  := xi_app_1 (beta lambda)
+    _ ~> (suc_c ⬝ (suc_c ⬝ 0))            := beta zero
+    _ ~> suc_c ⬝ 1                        := xi_app_2 lambda (beta zero)
+    _ ~> 2                                := beta (succ zero)
+
+example : two ~>> 2 := two_to_2
 
 inductive Progress : Γ ⊢ A → Type where
   | step :
-      (M ~> N) → Progress M
+      M ~> N → Progress M
   | done :
       Value V → Progress V
   deriving Repr
@@ -300,7 +304,7 @@ open Progress
 
 def progress : ∀ (M : ∅ ⊢ A), Progress M
   | (# x) => by contradiction
-  | (ƛ N) => done Value.lambda
+  | (ƛ N) => done lambda
   | (L ⬝ M) =>
       match progress L with
         | step L_to_L' => step (xi_app_1 L_to_L')
@@ -310,12 +314,12 @@ def progress : ∀ (M : ∅ ⊢ A), Progress M
               | done w =>
                   match v with
                     | Value.lambda => step (beta w)
-  | o => done Value.zero
+  | o => done zero
   | (M +1) =>
       match progress M with
         | step M_to_M' => step (xi_succ M_to_M')
-        | done v => done (Value.succ v)
-  | (switch L M N) =>
+        | done v => done (succ v)
+  | (casesOn L M N) =>
       match progress L with
         | step L_to_L' => step (xi_case L_to_L')
         | done v =>
@@ -342,19 +346,105 @@ def evaluate (n : Nat) (L : ∅ ⊢ A) : Steps L :=
     | Nat.zero => steps nil out_of_gas
     | Nat.succ n =>
         match progress L with
-          | Progress.done v => Steps.steps nil (done v)
+          | Progress.done v => steps nil (done v)
           | @Progress.step _ _ _ M L_to_M =>
               match evaluate n M with
-                | Steps.steps M_to_N f => Steps.steps (cons L L_to_M M_to_N) f
+                | steps M_to_N f => steps (cons L L_to_M M_to_N) f
+
+-- code below by Wojciech Nawrocki
+
+open Lean Elab Meta Command in
+elab tk:"#reduce_full" t:term : command => do
+  withoutModifyingEnv <| runTermElabM fun _ => Term.withDeclName `_reduce do
+    let e ← Term.elabTerm t none
+    Term.synthesizeSyntheticMVarsNoPostponing
+    let e ← Term.levelMVarToParam (← instantiateMVars e)
+    withTheReader Core.Context (fun ctx => { ctx with options := ctx.options.setBool `smartUnfolding false }) do
+      let e ← withTransparency (mode := TransparencyMode.all) <| Meta.reduce e (explicitOnly := false) (skipProofs := false) (skipTypes := false)
+      logInfoAt tk e
+
+open Lean PrettyPrinter Delaborator SubExpr in
+@[delab app.Hoskinson.reduce_many.cons]
+partial def reduce_many.delabCons : Delab := do
+  let e ← getExpr
+  guard $ e.isAppOfArity' ``reduce_many.cons 7
+  let L ← withNaryArg 4 delab
+  let M ← withNaryArg 2 delab
+  let r ← withNaryArg 5 delab
+  let steps ← withNaryArg 6 go
+  `(calc
+    $L ~> $M := $r
+    $steps*
+  )
+where go : DelabM (TSyntaxArray ``calcStep) := do
+  let e ← getExpr
+  if e.isAppOfArity' ``reduce_many.nil 3 then
+    return #[]
+  guard $ e.isAppOfArity' ``reduce_many.cons 7
+  let M ← withNaryArg 2 delab
+  let r ← withNaryArg 5 delab
+  let s ← `(calcStep|_ ~> $M := $r)
+  let rest ← withNaryArg 6 go
+  return #[s] ++ rest
 
 
 -- #eval two_plus_two
 -- #eval (evaluate 100 two_plus_two)
 
+#reduce_full two_to_2
 
-#reduce two_plus_two
-#reduce (evaluate 100 two_plus_two)
+#reduce_full two
+#reduce_full (evaluate 10 two)
 
+/-
+example :
+  (evaluate 10 two)
+      =
+      steps
+        (reduce_many.cons
+          ((ƛƛ#S Z⬝(#S Z⬝#Z))⬝(ƛ#Z+1)⬝o~>(ƛ(ƛ#Z+1)⬝((ƛ#Z+1)⬝#Z))⬝o)
+          ((beta Value.lambda).xi_app_1)
+          (reduce_many.cons
+            ((ƛ#Z+1)⬝((ƛ#Z+1)⬝o))
+            (beta Value.zero)
+            (reduce_many.cons
+              ((ƛ#Z+1)⬝o+1)
+              (xi_app_2 Value.lambda (beta Value.zero))
+              (reduce_many.cons
+                (o+1+1)
+                (beta Value.zero.succ)
+                reduce_many.nil))))
+        (Finished.done Value.zero.succ.succ)
+      :=
+        by rfl
+
+set_option pp.notation false
+
+example :
+  (evaluate 10 two)
+    =
+    steps
+      (calc
+        (ƛƛ#S Z⬝(#S Z⬝#Z))⬝(ƛ#Z+1)⬝o~>(ƛ(ƛ#Z+1)⬝((ƛ#Z+1)⬝#Z))⬝o := (beta Value.lambda).xi_app_1
+        _~>(ƛ#Z+1)⬝((ƛ#Z+1)⬝o) := (beta Value.zero)
+        _~>(ƛ#Z+1)⬝o+1 := (xi_app_2 Value.lambda (beta Value.zero))
+        _~>o+1+1 := beta Value.zero.succ)
+      (Finished.done Value.zero.succ.succ)
+    :=
+      by rfl
+
+-/
+
+#reduce_full two_plus_two
+#reduce_full (evaluate 100 two_plus_two)
+
+#check ((μƛƛcasesOn (#Z) (#S Z)
+                    ((#S
+                              S
+                                S
+                                  Z⬝#S
+                              S
+                                Z⬝#Z)+1))⬝o+1+1⬝o+1+1)
 
 -- Exercise. Add products, as detailed in
 --  https://plfa.inf.ed.ac.uk/More/#products
